vcg_seq_split done for now
git-svn-id: orca@236

WP1-Programming-Languages-Semantics/WP11-C-semantics/src/IMP-Lenses/hoare/VCG_total_ML.thy
@@ -4,43 +4,124 @@ theory VCG_total_ML
   imports utp_hoare_total
 begin
 
-lemmas subst_exp_thms = uop.abs_eq bop.abs_eq trop.abs_eq qtop.abs_eq subst.abs_eq
-lemmas simp_thms = lens_indep_def
+text \<open>@{text \<open>infixl\<close>} rather than @{text \<open>infixr\<close>} for @{text seq} may work better for tactics\<close>
+no_notation useq (infixr ";;" 51)
+notation useq (infixl ";;" 51)
+
+text \<open>@{thm seq_hoare_r_t} and @{thm assigns_hoare_r_t} are handled separately as they could cause
+conflicts/failed proofs later on.\<close>
+lemmas vcg_rules = skip_hoare_r_t cond_hoare_r_t assigns_hoare_r'_t assert_hoare_r_t
+assume_hoare_r_t while_invr_hoare_r_t while_hoare_r_t while_hoare_r'_t
+lemmas unfold_thms = lens_indep_def
+
+text \<open>Examples of breaking down theorems as terms\<close>
+ML \<open>
+val hoare_rd = @{thm hoare_rd_def};
+hoare_rd |> Thm.concl_of |> HOLogic.dest_Trueprop |> HOLogic.dest_eq |> fst;
+
+val seqr = @{thm seqr.rep_eq};
+seqr |> Thm.concl_of |> HOLogic.dest_Trueprop |> HOLogic.dest_eq |> fst;
+
+val rassume_c = @{thm rassume_c_def};
+rassume_c |> Thm.concl_of |> HOLogic.dest_Trueprop |> HOLogic.dest_eq |> fst
+\<close>
+
+(* Need to start with seq splitting, applying the `seq_hoare_r_t[of _ _ true]` step when an
+assumption is the last command in a goal; then we can apply other rules and such. When we encounter
+while loops and if statements we have to try seq splitting again after while/if application as those
+statements can have nested sequences of commands (including more while/if statements).
+Tricky tricky. *)
 
 (* FIRST' isn't necessary if you only have one tactic to try; it's meant for lists of tactics.
 However, it seems the below setups would need to be revised some other way to use without FIRST'.*)
 ML \<open>
-@{cterm "(1::nat) + 2"};
-let
-  val chead = @{cterm "P :: unit \<Rightarrow> nat \<Rightarrow> bool"}
-  val cargs = [@{cterm "()"}, @{cterm "3::nat"}]
-in
-  Drule.list_comb (chead, cargs)
-end;
+fun pprint_term ctxt term = Pretty.writeln (Syntax.pretty_term ctxt term)
+fun pprint_cterm ctxt cterm = pprint_term ctxt (Thm.term_of cterm)
+
+(* ML-level version of `seq_hoare_r_t[of _ _ true]`; there's also (Drule.)infer_instantiate', but
+that requires a proof context. *)
+val seq_hoare_r_t' =
+  Thm.instantiate' [SOME @{ctyp 'a}] [NONE, NONE, SOME @{cterm true}] @{thm seq_hoare_r_t}
+
+(* Splits up programs using seq_hoare_r_t; applies  `seq_hoare_r_t[of _ _ true]` when an assumption
+is the last command in a goal.
+Subgoal.focus elements: {prems, params, asms, concl, context, schematics} *)
+fun vcg_seq_split ctxt goal = (REPEAT o CHANGED) (Subgoal.FOCUS (fn {concl, ...} =>
+  case concl |> Thm.term_of |> HOLogic.dest_Trueprop of
+    Const (@{const_name hoare_rd}, _) $ _ $
+      (Const (@{const_name seqr}, _) $ _ $
+        (Const (@{const_name rassume_c}, _) $ _)) $
+    _ => resolve_tac ctxt [seq_hoare_r_t'] goal |
+    _ => resolve_tac ctxt @{thms seq_hoare_r_t} goal
+  ) ctxt goal)
+
+(* Handles applying most Hoare rules, with the specific exclusion of seq_hoare_r_t and
+assigns_hoare_r_t; match_tac (equivalent to `intro`) may be a better choice. *)
+(* fun vcg_resolve_tac ctxt = (ALLGOALS o REPEAT_ALL_NEW) (CHANGED o TRY o FIRST'
+                           [resolve_tac ctxt @{thms vcg_rules}]) *)
+fun vcg_resolve_tac ctxt goal = (REPEAT o CHANGED) (resolve_tac ctxt @{thms vcg_rules} goal)
 
 (* Equivalent to `apply (insert assms)`;
 not needed for rule application, only some {rel,pred}_* usage *)
-fun vcg_assms_insert_tac ctxt = (ALLGOALS o FIRST')
-                                [Method.insert_tac ctxt (Assumption.all_prems_of ctxt)];
+fun vcg_insert_assms_tac ctxt = (ALLGOALS o FIRST')
+                                [Method.insert_tac ctxt (Assumption.all_prems_of ctxt)]
 
-(* fun vcg_match_tac ctxt = (ALLGOALS o REPEAT_ALL_NEW) (CHANGED o TRY o FIRST'
-                         [match_tac ctxt @{thms (* vcg *)_}]); *)
-fun vcg_simp_tac ctxt = (ALLGOALS o asm_full_simp_tac) (ctxt addsimps @{thms simp_thms});
-fun vcg_subst_exp_tac ctxt = (ALLGOALS o REPEAT_ALL_NEW) (CHANGED o TRY o FIRST'
-                             [EqSubst.eqsubst_tac ctxt [0] @{thms subst_exp_thms}]);
+(* Must come before certain usages of {rel,pred}_*  *)
+fun vcg_unfold_tac ctxt = unfold_tac ctxt @{thms unfold_thms}
 
-val vcg_tac = (* vcg_match_tac THEN' *)
-              vcg_assms_insert_tac THEN'
-              vcg_simp_tac THEN'
-              vcg_subst_exp_tac THEN'
-              vcg_simp_tac;
+val vcg_tac =(*  vcg_resolve_tac THEN' *)
+              vcg_insert_assms_tac THEN'
+              (* apply rules, but with specific handling for the assumes/etc. cases;
+              may also want to stick with partial rule application so we can
+              do {pred,rel}_* on the way THEN' *)
+              vcg_unfold_tac (* THEN'
+              do stuff with {pred,rel}_* *)
+\<close>
 
-fun vcg_subst_tac ctxt = (ALLGOALS o REPEAT_ALL_NEW) (CHANGED o TRY o FIRST'
-                         [EqSubst.eqsubst_tac ctxt [0] @{thms (* vcg *)_}]);
+lemma increment_manual:
+  assumes "vwb_lens x" and "x \<bowtie> y"
+  shows
+  "\<lbrace>&y =\<^sub>u \<guillemotleft>5::int\<guillemotright>\<rbrace>
+  x \<Midarrow> 0;;
+  (&x =\<^sub>u 0 \<and> &y =\<^sub>u 5)\<^sup>\<top>\<^sup>C;;
+  while &x <\<^sub>u &y
+  invr &x \<le>\<^sub>u &y \<and> &y =\<^sub>u 5
+  do x \<Midarrow> &x + 1 od
+  \<lbrace>&x =\<^sub>u 5\<rbrace>\<^sub>D"
+  apply (insert assms)
+  apply (rule seq_hoare_r_t)
+   apply (rule seq_hoare_r_t[of _ _ true])
+    apply rel_auto (* seq rule gives us a value of true in postcondition, which is trivial *)
+   apply (rule assume_hoare_r_t)
+    apply (rule skip_hoare_r_t)
+   apply rel_auto
+  apply (rule while_invr_hoare_r_t)
+    apply (rule assigns_hoare_r_t)
+    unfolding lens_indep_def
+    apply pred_auto
+   apply pred_auto
+  apply pred_auto
+  done
 
-fun transfer_tac ctxt = ALLGOALS (Transfer.transfer_tac true ctxt);
+lemma increment_tactic:
+  assumes "vwb_lens x" and "x \<bowtie> y"
+  shows
+  "\<lbrace>&y =\<^sub>u \<guillemotleft>5::int\<guillemotright>\<rbrace>
+  x \<Midarrow> 0;;
+  (&x =\<^sub>u 0 \<and> &y =\<^sub>u 5)\<^sup>\<top>\<^sup>C;;
+  while &x <\<^sub>u &y
+  invr &x \<le>\<^sub>u &y \<and> &y =\<^sub>u 5
+  do x \<Midarrow> &x + 1 od
+  \<lbrace>&x =\<^sub>u 5\<rbrace>\<^sub>D"
+  apply (tactic \<open>vcg_seq_split @{context} 1\<close>)
+  apply rel_auto
+  apply (tactic \<open>vcg_resolve_tac @{context} 1\<close>)
+  apply rel_auto
+oops
 
-val hoare_solver_tac = transfer_tac THEN' vcg_simp_tac;
+ML \<open>
+@{term "\<lbrace>p\<rbrace>C;;a\<^sup>\<top>\<^sup>C\<lbrace>q\<rbrace>\<^sub>D"};
+pprint_cterm @{context} @{cterm "\<lbrace>p\<rbrace>C;;c\<^sup>\<top>\<^sup>C\<lbrace>q\<rbrace>\<^sub>D"}
 \<close>
 
 end
